tests/AddWithDelay/ListProofs.v
@@ -1,0 +1,123 @@
+(****************************************************************************)
+(* Copyright 2020 The Project Oak Authors                                   *)
+(*                                                                          *)
+(* Licensed under the Apache License, Version 2.0 (the "License")           *)
+(* you may not use this file except in compliance with the License.         *)
+(* You may obtain a copy of the License at                                  *)
+(*                                                                          *)
+(*     http://www.apache.org/licenses/LICENSE-2.0                           *)
+(*                                                                          *)
+(* Unless required by applicable law or agreed to in writing, software      *)
+(* distributed under the License is distributed on an "AS IS" BASIS,        *)
+(* WITHOUT WARRANTIES OR CONDITIONS OF ANY KIND, either express or implied. *)
+(* See the License for the specific language governing permissions and      *)
+(* limitations under the License.                                           *)
+(****************************************************************************)
+
+From Coq Require Import Arith.PeanoNat NArith.NArith Lists.List.
+Require Import Coq.micromega.Lia.
+Require Import Coq.Bool.Bvector.
+Import ListNotations.
+
+Require Import ExtLib.Structures.Monads.
+Export MonadNotation.
+
+Require Import coqutil.Tactics.Tactics.
+
+Require Import Cava.Cava.
+Require Import Cava.ListUtils.
+Require Import Cava.Tactics.
+Require Import Cava.Acorn.Acorn.
+Require Import Cava.Acorn.Identity.
+Require Import Cava.Acorn.SequentialProperties.
+Require Import Cava.Lib.UnsignedAdders.
+
+Require Import Tests.AddWithDelay.AddWithDelay.
+Local Open Scope nat_scope.
+
+Definition bvadd {n} (a b : Signal.combType (Vec Bit n)) : Signal.combType (Vec Bit n) :=
+  N2Bv_sized n (Bv2N a + Bv2N b).
+
+Definition bvzero {n} : Signal.combType (Vec Bit n) := N2Bv_sized n 0.
+
+Definition addWithDelaySpecF
+           (input : nat -> Signal.combType (Vec Bit 8)) : nat -> Signal.combType (Vec Bit 8) :=
+  fix out (t : nat) :=
+    match t with
+    | 0 => bvzero (* first round is just a delay *)
+    | 1 =>
+      (* second round is first input (because initial feedback = 0) *)
+      input 0
+    | S (S t') =>
+      (* if t > 2, out(t) = in(t-1) + out(t-2) *)
+      bvadd (input (S t')) (out t')
+    end.
+
+Definition addNSpec {n} (a b : seqType (Vec Bit n)) :=
+  map2 bvadd a b.
+
+Lemma addNCorrect n (a b : list (Bvector n)) :
+  sequential (addN (semantics:=SequentialCombSemantics) (a, b)) = addNSpec a b.
+Admitted.
+Hint Rewrite addNCorrect using solve [eauto] : seqsimpl.
+
+Lemma addWithDelayStepCorrect :
+  forall (i : Bvector 8) (s : Bvector 8),
+    sequential ((addN >=> delay >=> fork2) ([i], [s]))
+    = ([bvzero; bvadd i s], [bvzero; bvadd i s]).
+Proof.
+  intros. seqsimpl. reflexivity.
+Qed.
+Hint Rewrite addWithDelayStepCorrect using solve [eauto] : seqsimpl.
+
+Lemma Bv2N_bvzero n : Bv2N (@bvzero n) = 0%N.
+Proof.
+  cbv [bvzero N2Bv_sized Bvect_false].
+  induction n; intros; [ reflexivity | ].
+  rewrite const_cons. cbn [Bv2N].
+  rewrite IHn. reflexivity.
+Qed.
+
+Lemma bvadd_bvzero_l {n} (x : Bvector n) : bvadd x bvzero = x.
+Proof.
+  cbv [bvadd]. rewrite Bv2N_bvzero.
+  rewrite N.add_0_r, N2Bv_sized_Bv2N.
+  reflexivity.
+Qed.
+
+Lemma addWithDelayCorrect (i : list (Bvector 8)) :
+  sequential (addWithDelay i) = map (fun t => addWithDelaySpecF (fun n => nth n i bvzero) t)
+                                    (seq 0 (if length i =? 0 then 0 else S (length i))).
+Proof.
+  intros; cbv [addWithDelay].
+  eapply (loop_invariant_alt (B:=Vec Bit 8) (C:=Vec Bit 8))
+    with (I:=fun t acc feedback =>
+               0 < t
+               /\ feedback = [nth (t-1) acc bvzero; nth t acc bvzero]
+               /\ acc = map (fun t => addWithDelaySpecF
+                                    (fun n => nth n i bvzero) t) (seq 0 (S t))).
+  { (* invariant is satisfied at start *)
+    destruct i; [ ssplit; reflexivity | ].
+    seqsimpl. autorewrite with natsimpl.
+    cbn [nth map seq addWithDelaySpecF].
+    change (Signal.defaultCombValue (Vec Bit 8)) with (@bvzero 8).
+    rewrite bvadd_bvzero_l. ssplit; (reflexivity || lia). }
+  { (* invariant holds through loop *)
+    intros *. intros [Ht [Hfeedback Hacc]]. cbv zeta; intros.
+    subst. seqsimpl.
+    rewrite seq_S, map_app. cbn [map].
+    rewrite !overlap_snoc_cons by length_hammer.
+    autorewrite with push_nth push_length natsimpl.
+    cbn [nth]. ssplit; [ lia | reflexivity | ].
+    rewrite !seq_S, !map_app. cbn [map].
+    autorewrite with natsimpl. cbn [addWithDelaySpecF].
+    destruct t; [ lia | ].
+    rewrite !seq_S, !map_app. cbn [map].
+    autorewrite with natsimpl push_length push_nth.
+    cbn [nth]. rewrite <-!app_assoc.
+    reflexivity. }
+  { (* invariant implies postcondition *)
+    intros *; intros [Ht [Hfeedback Hacc]]; intros.
+    subst. destruct i; autorewrite with push_length in *; [ lia | ].
+    reflexivity. }
+Qed.
